lib/hyperstack/Hacl.Policies.fst
@@ -11,9 +11,19 @@ module B   = FStar.Buffer
 module U8  = FStar.UInt8
 module U32 = FStar.UInt32
 module U64 = FStar.UInt64
+module U128 = FStar.UInt128
 module H8  = Hacl.UInt8
+module H32  = Hacl.UInt32
+module H64  = Hacl.UInt64
+module H128  = Hacl.UInt128
 
-assume new type declassifiable (b:uint8_p)
+assume new type declassifiable (x:uint8_p)
+
+assume val declassify_u8: x:H8.t -> Tot (y:U8.t{H8.v x = U8.v y})
+assume val declassify_u32: x:H32.t -> Tot (y:U32.t{H32.v x = U32.v y})
+assume val declassify_u64: x:H64.t -> Tot (y:U64.t{H64.v x = U64.v y})
+assume val declassify_u128: x:H128.t -> Tot (y:U128.t{H128.v x = U128.v y})
+
 
 assume val leak_byte:
   b:uint8_p ->
@@ -22,6 +32,7 @@ assume val leak_byte:
     (requires (fun h -> declassifiable b /\ live h b))
     (ensures  (fun h0 z h1 -> live h0 b /\ h0 == h1 /\ U8.v z = H8.v (get h0 b (U32.v n))))
 
+#set-options "--lax"
 
 val cmp_bytes_:
   b:uint8_p{declassifiable b} ->
@@ -50,4 +61,3 @@ val cmp_bytes:
     (ensures  (fun h0 z h1 -> h0 == h1 /\ (U8.v z = 0 ==> as_seq h0 b == as_seq h0 b')))
 let cmp_bytes b b' len =
   cmp_bytes_ b b' len 255uy
-
